firmware/IncrementWait/CavaIncrementDevice.v
@@ -51,20 +51,22 @@ Section WithParameters.
 
   Global Instance counter_device: device := {|
     device.state := denote_type (state_of incr);
-    device.is_ready_state s := exists r_prev_state r_regs r_inner,
-        incr_invariant s (RSIdle, r_prev_state, r_regs, TLUL.Idle, r_inner);
+
+    device.is_ready_state s := exists r_regs r_tl r_inner,
+        incr_invariant s (RSIdle, r_regs, r_tl, r_inner);
+
     device.last_d2h '((_, (_, (_, d2h))), _) := d2h;
+
     device.tl_inflight_ops '((_, (_, (_, d2h))), _) :=
       if d_valid d2h then [d_source d2h] else [];
+
     device.run1 s i := fst (Semantics.step incr s (i, tt));
+
     device.addr_range_start := INCR_BASE_ADDR;
     device.addr_range_pastend := INCR_END_ADDR;
+
     device.maxRespDelay '((_, (_, (_, d2h))), _) :=
-      if a_ready d2h then 2
-      else if d_valid d2h then 1
-           else 0;
-    (* The last [else] is not reachable, because [d_valid] is always the
-       negation of [a_ready]. *)
+      if a_ready d2h then 0 else 1;
   |}.
 
   (* conservative upper bound matching the instance given in IncrementWaitToRiscv *)
@@ -72,58 +74,25 @@ Section WithParameters.
   {| ncycles_processing := 15%nat |}.
 
 
-  Inductive counter_related_base: IncrementWaitSemantics.state -> Incr.repr_state -> Incr.inner_state -> Prop :=
-  | IDLE_related: forall r_innr,
-      counter_related_base IDLE RSIdle r_innr
-  | BUSY1_related: forall val ncycles,
-      (1 < ncycles)%nat ->
-      counter_related_base (BUSY val ncycles) (RSBusy (word_to_N val))
-                           (IISBusy (word_to_N val) 1)
-  | BUSY2_related: forall val ncycles,
-      (0 < ncycles)%nat ->
-      counter_related_base (BUSY val ncycles) (RSBusy (word_to_N val))
-                           (IISBusy (word_to_N val) 2)
+  Inductive counter_related_spec: IncrementWaitSemantics.state -> Incr.repr_state -> Prop :=
+  | IDLE_related: counter_related_spec IDLE RSIdle
+  | BUSY_related: forall val ncycles count,
+      (0 < count <= 2)%nat ->
+      (2 < ncycles + count)%nat ->
+      counter_related_spec (BUSY val ncycles) (RSBusy (word_to_N val) count)
   (* the hardware is already done, but the software hasn't polled it yet to find out,
      so we have to relate a software-BUSY to a hardware-done: *)
-  | BUSY_done_related: forall val ncycles r_innr,
-      counter_related_base (BUSY val ncycles) (RSDone (word_to_N (word.add (word.of_Z 1) val))) r_innr
-  | DONE_related: forall val r_innr,
-      counter_related_base (DONE val) (RSDone (word_to_N val)) r_innr.
-
-  Inductive counter_related_spec: IncrementWaitSemantics.state -> repr ->
-                                  list tl_h2d -> Prop :=
-  | No_inflight: forall sH r_state r_prev_state r_regs r_inner,
-      counter_related_base sH r_state r_inner ->
-      counter_related_spec sH (r_state, r_prev_state, r_regs, TLUL.Idle, r_inner) []
-  | Inflight_read_status: forall sH r_state r_prev_state r_regs r_tl r_tl_regs r_inner h2d,
-      counter_related_base sH r_state r_inner ->
-      r_tl = TLUL.OutstandingAccessAckData (set_a_address 4 h2d) r_tl_regs ->
-      a_valid h2d = true ->
-      a_opcode h2d = Get ->
-      a_address h2d = word_to_N (state_machine.reg_addr STATUS) ->
-      counter_related_spec sH (r_state, r_prev_state, r_regs, r_tl, r_inner) [h2d]
-  | Inflight_read_value: forall r_prev_state r_regs r_tl r_tl_regs r_inner val h2d,
-      r_tl = TLUL.OutstandingAccessAckData (set_a_address 0 h2d) r_tl_regs ->
-      nth 0 r_tl_regs 0%N = word_to_N val ->
-      a_valid h2d = true ->
-      a_opcode h2d = Get ->
-      a_address h2d = word_to_N (state_machine.reg_addr VALUE) ->
-      counter_related_spec (DONE val)
-                           (RSIdle, r_prev_state, r_regs, r_tl, r_inner)
-                           [h2d]
-  | Inflight_write_value: forall r_prev_state r_regs r_tl r_inner val h2d,
-      r_tl = TLUL.OutstandingAccessAck (set_a_address 0 h2d) ->
-      a_valid h2d = true ->
-      a_opcode h2d = PutFullData ->
-      a_address h2d = word_to_N (state_machine.reg_addr VALUE) ->
-      a_data h2d = (word_to_N val) ->
-      counter_related_spec (IDLE)
-                           (RSBusy (word_to_N val), r_prev_state, r_regs, r_tl, r_inner)
-                           [h2d].
+  | BUSY_done_related: forall val ncycles,
+      counter_related_spec (BUSY val ncycles) (RSDone (word_to_N (word.add (word.of_Z 1) val)))
+  | DONE_related: forall val,
+      counter_related_spec (DONE val) (RSDone (word_to_N val)).
 
   Definition counter_related {invariant : invariant_for incr repr} (sH : IncrementWaitSemantics.state)
              (sL : denote_type (state_of incr)) (inflight_h2ds : list tl_h2d) : Prop :=
-    exists repr, counter_related_spec sH repr inflight_h2ds /\ invariant sL repr.
+    exists r_state r_regs r_tl r_inner,
+      inflight_h2ds = [] /\
+      counter_related_spec sH r_state /\
+      invariant sL (r_state, r_regs, r_tl, r_inner).
 
   (* This should be in bedrock2.ZnWords. It is use by ZnWords, which is used in
      the two following Lemmas. *)
@@ -137,62 +106,8 @@ Section WithParameters.
       (0 <= x < 2 ^ 32)%Z -> word_to_N (word.of_Z x) = Z.to_N x.
   Proof. intros. unfold word_to_N. ZnWords. Qed.
 
-  Set Printing Depth 100000.
-
-  Ltac destruct_pair_let_hyp :=
-    match goal with
-    | H: context [ match ?p with
-                   | pair _ _ => _
-                   end ] |- _ =>
-      destruct p as [?p0 ?p1] eqn:?H0
-    end.
-
-  Ltac destruct_pair_equal_hyp :=
-    match goal with
-    | H: context [ (?l0, ?l1) = (?r0, ?r1) ] |- _ =>
-      eapply pair_equal_spec in H; destruct H as [?H0 ?H1]
-    end.
-
   Lemma N_to_word_word_to_N: forall v, N_to_word (word_to_N v) = v.
   Proof. intros. unfold N_to_word, word_to_N. ZnWords. Qed.
-
-(* TODO move to coqutil *)
-Ltac contradictory H :=
-  lazymatch type of H with
-  | ?x <> ?x => exfalso; apply (H eq_refl)
-  | False => case H
-  end.
-
-Require Import coqutil.Tactics.autoforward.
-
-Ltac fwd_step ::=
-  match goal with
-  | H: ?T |- _ => is_destructible_and T; destr_and H
-  | H: exists y, _ |- _ => let yf := fresh y in destruct H as [yf H]
-  | H: ?x = ?x |- _ => clear H
-  | H: True |- _ => clear H
-  | H: ?LHS = ?RHS |- _ =>
-    let h1 := head_of_app LHS in is_constructor h1;
-    let h2 := head_of_app RHS in is_constructor h2;
-    (* if not eq, H is a contradiction, but we don't want to change the number
-       of open goals in this tactic *)
-    constr_eq h1 h2;
-    (* we don't use `inversion H` or `injection H` because they unfold definitions *)
-    inv_rec LHS RHS;
-    clear H
-  | E: ?x = ?RHS |- context[match ?x with _ => _ end] =>
-    let h := head_of_app RHS in is_constructor h; rewrite E in *
-  | H: context[match ?x with _ => _ end], E: ?x = ?RHS |- _ =>
-    let h := head_of_app RHS in is_constructor h; rewrite E in *
-  | H: context[match ?x with _ => _ end] |- _ =>
-    (* note: recursive invocation of fwd_step for contradictory cases *)
-    destr x; try solve [repeat fwd_step; contradictory H]; []
-  | H: _ |- _ => autoforward with typeclass_instances in H
-  | |- _ => progress subst
-  | |- _ => progress fwd_rewrites
-  end.
-
-  Axiom TODO: False.
 
   Ltac use_spec :=
     match goal with
@@ -200,33 +115,54 @@ Ltac fwd_step ::=
             Hinv: incr_invariant ?sL ?repr
       |- _ =>
       assert (Hprec: precondition incr (input, tt) repr);
-      [|
-       (* pose proof (output_correct_pf (c:=incr) (input, tt) sL repr Hinv Hprec) as Hpostc. *)
-       remember (update_repr (c:=incr) (input, tt) repr) as repr' eqn:Erepr';
-       pose proof (invariant_preserved_pf (c:=incr) (input, tt) sL repr repr' Erepr' Hinv Hprec) as Hinv';
-       unfold device.run1, counter_device in Hrun;
-       match type of Hrun with
-       | fst ?step = _ =>
-         remember step as res eqn:Hstep;
-         destruct res as (?sL'' & ?d2h);
-         cbn in Hrun; subst sL''; clear Hstep
-       end;
-       cbn [fst] in Hinv']
+      [ simplify_spec (incr (var:=var)); simplify_spec (tlul_adapter_reg (reg_count:=2)); simplify_spec (Incr.inner (var:=var));
+        simplify_invariant (incr (var:=var));
+        cbn in sL; destruct sL as ((?busy, (?done, (?regs, ?d2h))), (?s_tl, ?s_inner));
+        destruct_tl_h2d; tlsimpl; logical_simplify; subst;
+        ssplit; intros; try discriminate; auto
+
+      | remember (update_repr (c:=incr) (input, tt) repr) as repr' eqn:Erepr';
+        (* pose proof (output_correct_pf (c:=incr) (input, tt) sL repr Hinv Hprec) as Hpostc. *)
+        pose proof (invariant_preserved_pf (c:=incr) (input, tt) sL repr repr' Erepr' Hinv Hprec) as Hinv';
+        unfold device.run1, counter_device in Hrun;
+        match type of Hrun with
+        | fst ?step = _ =>
+          remember step as res eqn:Hstep;
+          destruct res as (?sL'' & ?d2h);
+          cbn in Hrun; subst sL''; clear Hstep
+        end;
+        cbn [fst] in Hinv';
+        destruct repr' as (((?r_state, ?r_regs), ?r_tl), ?r_inner)]
     end.
 
   Ltac inversion_rel_spec :=
     match goal with
-    | H: counter_related_spec _ _ _ |- _ => inversion H; subst
-    end.
-  Ltac inversion_rel_base :=
-    match goal with
-    | H: counter_related_base _ _ _ |- _ => inversion H; subst
+    | H: counter_related_spec _ _ |- _ => inversion H; subst
     end.
 
-  (* Lemma output_last_d2h : forall s h2d s' d2h, *)
-  (*     (s', d2h) = Semantics.step incr s (h2d, tt) -> *)
-  (*     device.last_d2h s' = d2h. *)
-  (* Proof. *)
+  Ltac simplify_tl_repr :=
+    unfold device.maxRespDelay, device.last_d2h, counter_device in *;
+    repeat match goal with
+    | sL: device.state |- _ =>
+      cbn in sL; destruct sL as ((?busy, (?done, (?regs, ?d2h))), (?s_tl, ?s_inner))
+    end;
+    destruct_tl_h2d; destruct_tl_d2h; tlsimpl; logical_simplify; subst;
+    simplify_invariant (incr (var:=var));
+    match goal with
+    | H: _ = update_repr _ (_, _, ?r_tl, _) |- _ =>
+      destruct r_tl; logical_simplify; tlsimpl; subst;
+      (* logical_simplify; subst; *)
+      cbn in H; rewrite ? Z_word_N in H by lia; cbn in H
+    end;
+    logical_simplify; subst;
+    cbn; rewrite ? Z_word_N by lia; cbn;
+    change (Pos.to_nat 1) with 1;
+    repeat match goal with
+    | H: length ?regs = 2 |- _ =>
+      destruct regs as [|? [|? [|]]]; cbn in H; try discriminate H; clear H;
+      cbn [nth] in *; subst
+    end;
+    try discriminate.
 
   Global Instance cava_counter_satisfies_state_machine:
     device_implements_state_machine counter_device increment_wait_state_machine.
@@ -235,323 +171,136 @@ Ltac fwd_step ::=
     - (* mmioAddrs_match: *)
       reflexivity.
     - (* initial_state_is_ready_state: *)
-      intros ? ? ? Hrel.
-      cbn in *. subst. destruct Hrel as [?repr [?Hrel ?Hinv]].
-      inversion_rel_spec. inversion_rel_base.
-      repeat eexists. eapply Hinv.
+      intros.
+      unfold device.is_ready_state, counter_device, counter_related in *;
+        logical_simplify.
+      cbn in *; subst.
+      inversion_rel_spec; repeat eexists; eassumption.
     - (* initial_states_are_related: *)
-      intros ? ? ? Hready.
-      cbn in *. destruct Hready as (?r_prev_state & ?r_regs & ?r_inner & ?Hinv). subst.
-      unfold counter_related. eexists. split; [|apply Hinv].
-      apply No_inflight, IDLE_related.
+      intros.
+      cbn in *; logical_simplify; subst.
+      unfold counter_related; repeat eexists; [|eassumption].
+      apply IDLE_related.
     - (* initial_state_exists: *)
-      intros ? Hready.
-      cbn in *. destruct Hready as (?r_prev_state & ?r_regs & ?r_inner & ?Hinv).
-      eexists. split; [reflexivity|].
-      unfold counter_related. eexists. split; [|apply Hinv].
-      apply No_inflight, IDLE_related.
+      intros.
+      cbn in *; logical_simplify; subst.
+      unfold counter_related; repeat eexists; [|eassumption].
+      apply IDLE_related.
     - (* nonMMIO_device_step_preserves_state_machine_state: *)
-      intros ? ? ? ? Ha_valid [repr [Hrel Hinv]] **.
-      use_spec.
-      { destruct_tl_h2d. destruct_tl_d2h. tlsimpl.
-        cbn in sL1; destruct sL1 as ((?busy, (?done, (?regs, ?d2h))), (?s_tl, ?s_inner)).
-        destruct repr as ((((?r_state, ?r_prev_state), ?r_regs), ?r_tl), ?r_inner).
-        simplify_invariant incr. logical_simplify.
-        subst. cbn. ssplit; intros; [auto|discriminate|auto].
-      }
-      exists repr'; split; [|auto].
-      inversion_rel_spec; inversion_rel_base;
-        destruct_tl_h2d; destruct_tl_d2h; tlsimpl; subst;
-          cbn in sL1; destruct sL1 as ((?busy, (?done, (?regs, ?d2h))), (?s_tl, ?s_inner));
-            simplify_invariant incr; logical_simplify; subst; cbn -[replace];
-              apply No_inflight; try (constructor; lia); [].
-      replace ((word_to_N val + 1) mod 4294967296)%N with
-          (word_to_N (word.add (word.of_Z 1) val)) by
-          (unfold word_to_N; ZnWords);
-        apply BUSY_done_related.
+      intros.
+      logical_simplify.
+      unfold counter_related in *; logical_simplify.
+      use_spec. clear Hprec.
+      repeat eexists; [|eassumption].
+      inversion_rel_spec; simplify_tl_repr;
+        destruct d_ready; logical_simplify; subst; try constructor;
+          (destruct count as [|[|[|]]]; [exfalso; lia|..|exfalso; lia]);
+          rewrite ? incrN_word_to_bv; constructor; lia.
 
     - (* [state_machine_read_to_device_send_read_or_later] *)
-      intros ? ? ? ? ? ? [v [sH'' Hex_read]] [repr [Hrel Hinv]] **.
-      cbn in Hex_read. logical_simplify.
-      rewrite H5. clear H5.
-      use_spec.
-      1: simplify_spec incr; simplify_spec (tlul_adapter_reg (reg_count:=2)); simplify_spec Incr.inner;
-        simplify_invariant incr;
-        cbn in sL; destruct sL as ((?busy, (?done, (?regs, ?d2h))), (?s_tl, ?s_inner));
-          destruct repr as ((((?r_state, ?r_prev_state), ?r_regs), ?r_tl), ?r_inner);
-          destruct_tl_h2d; tlsimpl; logical_simplify; subst;
-            ssplit; intros; auto.
+      intros ? ? ? ? ? ? [v [sH'' [Hpow2 Hex_read]]] **.
+      rewrite Hpow2. clear Hpow2.
+      unfold counter_related in *. cbn in Hex_read. logical_simplify.
+      use_spec. clear Hprec.
 
       destruct_one_match; [destruct_one_match|].
-      (* case 1: device ready, valid response
-           In our TL implementation [a_ready = negb d_valid], hence this case
-           is not possible.
-           case 3: device not ready
-           If the inflight queue is empty, the device must be ready, hence
-           this case is not possible. *)
-      1,3: exfalso;
-        unfold device.last_d2h, counter_device in *;
-        cbn in sL; destruct sL as ((?busy, (?done, (?regs, ?d2h))), (?s_tl, ?s_inner));
-          destruct repr as ((((?r_state, ?r_prev_state), ?r_regs), ?r_tl), ?r_inner);
-          simplify_invariant incr; subst; logical_simplify; destruct_tl_d2h; tlsimpl; subst;
-          inversion_rel_spec; logical_simplify; discriminate.
-      (* device ready, no valid response: *)
-      ssplit.
-      1: eexists; split; [|eassumption]; [].
-      all:
-        unfold device.tl_inflight_ops, device.last_d2h, device.maxRespDelay,
-        counter_device, counter_related in *;
-        cbn in sL; destruct sL as ((?busy, (?done, (?regs, ?d2h))), (?s_tl, ?s_inner));
-          cbn in sL'; destruct sL' as ((?busy, (?done, (?regs, ?d2h))), (?s_tl, ?s_inner));
-            destruct repr as ((((?r_state, ?r_prev_state), ?r_regs), ?r_tl), ?r_inner);
-            destruct_tl_d2h; destruct_tl_h2d;
-              simplify_spec incr; simplify_spec (tlul_adapter_reg (reg_count:=2));
-                simplify_invariant incr;
-                logical_simplify; tlsimpl; subst;
-                  cbn in Hinv'; logical_simplify; subst.
-      + destruct r.
-        * (* [r:=VALUE] *)
-          inversion_rel_spec; inversion_rel_base; destruct H6; subst.
-          cbn; replace (N.land (word_to_N (word.of_Z 16384)) 4) with 0%N
-            by (rewrite Z_word_N by lia; reflexivity);
-          cbn; eapply Inflight_read_value; [eauto| |reflexivity..].
-          logical_simplify. assumption.
-        * (* [r:=STATUS] *)
-          inversion_rel_spec; inversion_rel_base; subst; logical_simplify; subst; cbn.
-            eapply Inflight_read_status; try (constructor; lia).
-          all: replace (N.land (word_to_N (word.of_Z 16388)) 4) with 4%N
-            by (rewrite Z_word_N by lia; reflexivity); eauto.
-          all: cbn; replace ((word_to_N val + 1) mod 4294967296)%N with
-                        (word_to_N (word.add (word.of_Z 1) val)) by
-              (unfold word_to_N; ZnWords); constructor.
+      { (* case 1: device ready, valid response *)
+        destruct r.
+        - (* [r:=VALUE] *)
+          inversion_rel_spec; destruct Hex_read; subst.
+          eexists; split; [|cbn; ssplit; try reflexivity].
+          + repeat eexists; [|eassumption].
+            simplify_tl_repr; constructor.
+          + simplify_tl_repr.
+            apply N_to_word_word_to_N.
+        - (* [r:=STATUS] *)
+          inversion_rel_spec.
+          + eexists; split; [repeat eexists; [|eassumption]|cbn; ssplit; try reflexivity];
+              simplify_tl_repr.
+            * constructor.
+            * unfold N_to_word, status_value; ZnWords.
 
-      + inversion_rel_spec; inversion_rel_base; subst; logical_simplify; subst; lia.
+          + destruct ncycles as [|]; [exfalso; lia|].
+            eexists; split; [repeat eexists; [|eassumption]|cbn; ssplit; try reflexivity];
+              simplify_tl_repr.
+            * destruct count as [|[|[|]]]; [exfalso; lia|..|exfalso; lia].
+              -- apply BUSY_related with (ncycles:=ncycles); lia.
+              -- rewrite incrN_word_to_bv; apply BUSY_done_related.
+            * right. eexists; ssplit; try reflexivity.
+              unfold N_to_word, status_value; ZnWords.
+
+          + eexists; split; [repeat eexists; [|eassumption]|cbn; ssplit; try reflexivity];
+              simplify_tl_repr.
+            * apply DONE_related.
+            * left. split; [|reflexivity].
+              unfold N_to_word, status_value; ZnWords.
+
+          + eexists; split; [repeat eexists; [|eassumption]|cbn; ssplit; try reflexivity];
+              simplify_tl_repr.
+            * apply DONE_related.
+            * unfold N_to_word, status_value; ZnWords.
+      }
+
+      { (* case 2: device ready, no valid response *)
+        exfalso; simplify_tl_repr.
+      }
+
+      { (* case 3: device not ready *)
+        ssplit.
+        - repeat eexists; [|eassumption].
+          inversion_rel_spec; simplify_tl_repr;
+            rewrite ? incrN_word_to_bv; try (constructor; lia).
+          all: destruct count as [|[|[|]]]; [exfalso; lia
+                                            |apply BUSY_related with (ncycles:=ncycles); lia
+                                            |apply BUSY_done_related
+                                            |exfalso; lia].
+        - simplify_tl_repr; lia.
+      }
 
     - (* [state_machine_read_to_device_ack_read_or_later] *)
-      intros ? ? ? ? ? ? [v [sH'' Hex_read]] [repr [Hrel Hinv]] **.
-      (* assert (Hex_rel: exists sL'' h2d', device.run1 sL'' (set_d_ready true h2d') = sL /\ *)
-      (*                               counter_related sH sL'' []). *)
-      (* { admit. } *)
-      (* logical_simplify. destruct H0 as [repr'' [Hrel'' Hinv'']]. *)
-      (* use_spec. 1: admit. *)
-      (* rename Hprec into Hprec''. rename repr' into repr'''. rename Erepr' into Erepr''. rename Hinv' into Hinv'''. *)
-      cbn in Hex_read. logical_simplify.
-      rewrite H2. clear H2. rename H3 into Hex_read.
-      use_spec.
-      1: simplify_spec incr; simplify_spec (tlul_adapter_reg (reg_count:=2)); simplify_spec Incr.inner;
-        simplify_invariant incr;
-        cbn in sL; destruct sL as ((?busy, (?done, (?regs, ?d2h))), (?s_tl, ?s_inner));
-          destruct repr as (((?r_state, ?r_regs), ?r_tl), ?r_inner);
-          destruct r_state;
-          destruct_tl_h2d; tlsimpl; logical_simplify; subst;
-            ssplit; intros; auto.
-
-      destruct_one_match.
-      (* case 2: no valid response
-         If the inflight queue is not empty, the device must be sending a
-         response, hence this case is not possible. *)
-      2: unfold device.last_d2h, counter_device in *;
-        cbn in sL; destruct sL as ((?busy, (?done, (?regs, ?d2h))), (?s_tl, ?s_inner));
-          destruct repr as (((?r_state, ?r_regs), ?r_tl), ?r_inner);
-          simplify_invariant incr; subst; logical_simplify; destruct_tl_d2h; tlsimpl; subst;
-            inversion_rel_spec; try inversion_rel_base; logical_simplify; subst;
-              try destruct r_tl; logical_simplify; subst;
-                discriminate.
-
-      (* case 1: valid response *)
-      destruct r.
-      + (* [r:=VALUE] *)
-        inversion_rel_spec;
-          try (exfalso; destruct_tl_h2d; tlsimpl; subst; unfold word_to_N in *; cbn in *; ZnWords).
-
-        destruct Hex_read; subst.
-        logical_simplify; subst.
-        exists IDLE. ssplit.
-        * eexists. split; [|eassumption].
-          cbn.
-          cbn in sL; destruct sL as ((?busy, (?done, (?regs, ?d2h))), (?s_tl, ?s_inner));
-            simplify_invariant incr;
-            logical_simplify; tlsimpl; subst.
-          apply No_inflight, IDLE_related.
-        * cbn. ssplit; try reflexivity.
-          clear Hinv'.
-          cbn in sL; destruct sL as ((?busy, (?done, (?regs, ?d2h))), (?s_tl, ?s_inner));
-          simplify_invariant incr.
-          logical_simplify; subst.
-          destruct_tl_h2d; tlsimpl; subst.
-          rewrite H19. cbn. rewrite H3. apply N_to_word_word_to_N.
-      + (* [r:=STATUS] *)
-        inversion_rel_spec;
-          try (exfalso; destruct_tl_h2d; tlsimpl; subst; unfold word_to_N in *; cbn in *; ZnWords).
-
-        inversion_rel_base;
-          cbn in sL |- *; destruct sL as ((?busy, (?done, (?regs, ?d2h))), (?s_tl, ?s_inner));
-            simplify_invariant incr;
-            logical_simplify; subst; logical_simplify; subst;
-              match goal with
-              | H: d_data _ = _ |- _ =>
-                rewrite H
-              end;
-              cbn; destruct_tl_h2d; tlsimpl; subst; cbn;
-              change (Pos.to_nat 1) with 1.
-                (* match goal with *)
-                (* | H: nth 1 r_tl_regs 0%N = _ |- _ => rewrite H *)
-                (* end; *)
-                (* unfold N_to_word, status_value. *)
-        * eexists; ssplit; try reflexivity.
-          -- eexists.
-             ssplit; [|eassumption].
-             apply No_inflight. constructor.
-          -- assert (Hprev: r_prev_state = RSIdle) by admit.
-             subst.
-             match goal with
-             | H: nth 1 r_tl_regs 0%N = _ |- _ => rewrite H
-             end; unfold N_to_word, status_value.
-             ZnWords.
-        * destruct ncycles as [|ncycles]; [lia|].
-          eexists; ssplit; try reflexivity.
-          -- eexists. ssplit; [|eassumption].
-             apply No_inflight, BUSY2_related. apply lt_S_n. eauto.
-          -- right. eexists. ssplit; [reflexivity| |reflexivity].
-             assert (Hprev: exists d, r_prev_state = RSBusy d) by admit.
-             logical_simplify; subst.
-             match goal with
-             | H: nth 1 r_tl_regs 0%N = _ |- _ => rewrite H
-             end; unfold N_to_word, status_value.
-             ZnWords.
-        * destruct ncycles as [|ncycles]; [lia|].
-          eexists. ssplit; try reflexivity.
-          -- eexists. ssplit; [|eassumption].
-             cbn; rewrite incrN_word_to_bv.
-             apply No_inflight, BUSY_done_related.
-          -- right. eexists. ssplit; [reflexivity| |reflexivity].
-             assert (Hprev: exists d, r_prev_state = RSBusy d) by admit.
-             logical_simplify; subst.
-             match goal with
-             | H: nth 1 r_tl_regs 0%N = _ |- _ => rewrite H
-             end; unfold N_to_word, status_value.
-             ZnWords.
-        * eexists; ssplit; try reflexivity.
-          -- eexists. ssplit; [|eassumption].
-             apply No_inflight, DONE_related.
-          -- left. ssplit; [|reflexivity].
-             assert (Hprev: exists d, r_prev_state = RSDone d) by admit.
-             logical_simplify; subst; logical_simplify;
-             match goal with
-             | H: nth 1 r_tl_regs 0%N = _ |- _ => rewrite H
-             end; unfold N_to_word, status_value.
-             ZnWords.
-        * eexists; ssplit; try reflexivity.
-          -- eexists. ssplit; [|eassumption].
-             apply No_inflight, DONE_related.
-          -- assert (Hprev: exists d, r_prev_state = RSDone d) by admit.
-             logical_simplify; subst; logical_simplify.
-             match goal with
-             | H: nth 1 r_tl_regs 0%N = _ |- _ => rewrite H
-             end; unfold N_to_word, status_value.
-             ZnWords.
+      intros.
+      unfold counter_related in *; logical_simplify.
+      discriminate.
 
     - (* [state_machine_write_to_device_send_write_or_later] *)
-      intros ? ? ? ? ? ? ? [sH'' [Hpow2 Hex_write]] [repr [Hrel Hinv]] **.
+      intros ? ? ? ? ? ? ? [sH'' [Hpow2 Hex_write]] **.
       rewrite Hpow2. clear Hpow2.
-      use_spec.
-      1: simplify_spec incr; simplify_spec (tlul_adapter_reg (reg_count:=2)); simplify_spec Incr.inner;
-        simplify_invariant incr;
-        cbn in sL; destruct sL as ((?busy, (?done, (?regs, ?d2h))), (?s_tl, ?s_inner));
-          destruct repr as ((((?r_state, ?r_prev_state), ?r_regs), ?r_tl), ?r_inner);
-          destruct_tl_h2d; tlsimpl; logical_simplify; subst;
-            ssplit; intros; auto.
-
+      unfold counter_related in *. logical_simplify.
+      use_spec. clear Hprec.
       destruct_one_match; [destruct_one_match|].
-        (* case 1: device ready, valid response
-           In our TL implementation [a_ready = negb d_valid], hence this case
-           is not possible.
-           case 3: device not ready
-           If the inflight queue is empty, the device must be ready, hence
-           this case is not possible. *)
-      1,3: exfalso;
-        unfold device.last_d2h, counter_device in *;
-        cbn in sL; destruct sL as ((?busy, (?done, (?regs, ?d2h))), (?s_tl, ?s_inner));
-        destruct repr as ((((?r_state, ?r_prev_state), ?r_regs), ?r_tl), ?r_inner);
-          simplify_invariant incr; subst; logical_simplify; destruct_tl_d2h; tlsimpl; subst;
-            inversion_rel_spec; logical_simplify; discriminate.
-      (* device ready, no valid response: *)
-      ssplit.
-      1: eexists; split; [|eassumption]; [].
-      all:
-        unfold device.tl_inflight_ops, device.last_d2h, device.maxRespDelay,
-        counter_device, counter_related in *;
-        cbn in sL; destruct sL as ((?busy, (?done, (?regs, ?d2h))), (?s_tl, ?s_inner));
-          cbn in sL'; destruct sL' as ((?busy, (?done, (?regs, ?d2h))), (?s_tl, ?s_inner));
-            destruct repr as ((((?r_state, ?r_prev_state), ?r_regs), ?r_tl), ?r_inner);
-            destruct_tl_d2h; destruct_tl_h2d;
-              simplify_spec incr; simplify_spec (tlul_adapter_reg (reg_count:=2));
-                simplify_invariant incr;
-                logical_simplify; tlsimpl; subst;
-                  cbn in Hinv'; logical_simplify; subst.
-      + destruct r.
-        * (* [r:=VALUE] *)
-          inversion_rel_spec; inversion_rel_base; logical_simplify; subst; try contradiction.
-          cbn. apply Inflight_write_value; eauto; [].
-          rewrite Z_word_N by lia. change (Z.to_N 16384) with 16384%N. reflexivity.
-        * (* [r:=STATUS] *)
-          inversion_rel_spec; inversion_rel_base;
+
+      { (* case 1: device ready, valid response *)
+        destruct r.
+        + (* [r:=VALUE] *)
+          inversion_rel_spec; destruct Hex_write; subst.
+          eexists; split; [|cbn; ssplit; try reflexivity].
+          repeat eexists; [|eassumption].
+          simplify_tl_repr; constructor; lia.
+        + (* [r:=STATUS] *)
           destruct Hex_write.
-      + inversion_rel_spec; inversion_rel_base; subst; logical_simplify; subst; lia.
+      }
+
+      { (* case 2: device ready, no valid response *)
+        exfalso; simplify_tl_repr.
+      }
+
+      { (* case 3: device not ready *)
+        ssplit.
+        - repeat eexists; [|eassumption].
+          inversion_rel_spec; simplify_tl_repr;
+            rewrite ? incrN_word_to_bv; try (constructor; lia).
+          all: destruct count as [|[|[|]]]; [exfalso; lia
+                                            |apply BUSY_related with (ncycles:=ncycles); lia
+                                            |apply BUSY_done_related
+                                            |exfalso; lia].
+        - simplify_tl_repr; lia.
+      }
 
     - (* [state_machine_write_to_device_ack_write_or_later] *)
-      intros ? ? ? ? ? ? ? [sH'' [Hpow2 Hex_write]] [repr [Hrel Hinv]] **.
-      rewrite Hpow2 in *. clear Hpow2.
-      use_spec.
-      1: simplify_spec incr; simplify_spec (tlul_adapter_reg (reg_count:=2)); simplify_spec Incr.inner;
-        simplify_invariant incr;
-        cbn in sL; destruct sL as ((?busy, (?done, (?regs, ?d2h))), (?s_tl, ?s_inner));
-          destruct repr as ((((?r_state, ?r_prev_state), ?r_regs), ?r_tl), ?r_inner);
-          destruct_tl_h2d; tlsimpl; logical_simplify; subst;
-            ssplit; intros; auto.
+      intros.
+      unfold counter_related in *; logical_simplify.
+      discriminate.
 
-      destruct_one_match.
-      (* case 2: no valid response
-         If the inflight queue is not empty, the device must be sending a
-         response, hence this case is not possible. *)
-      2: unfold device.last_d2h, counter_device in *;
-        cbn in sL; destruct sL as ((?busy, (?done, (?regs, ?d2h))), (?s_tl, ?s_inner));
-          destruct repr as ((((?r_state, ?r_prev_state), ?r_regs), ?r_tl), ?r_inner);
-          simplify_invariant incr; subst; logical_simplify; destruct_tl_d2h; tlsimpl; subst;
-            inversion_rel_spec; try inversion_rel_base; logical_simplify; subst;
-              try destruct r_tl; logical_simplify; subst;
-                discriminate.
-
-      (* case 1: valid response *)
-      destruct r.
-      + (* [r:=VALUE] *)
-        inversion_rel_spec;
-          try (exfalso; destruct_tl_h2d; tlsimpl; subst; unfold word_to_N in *; cbn in *; ZnWords).
-
-        destruct Hex_write; subst.
-        logical_simplify; subst.
-        eexists. ssplit; [|cbn; split; reflexivity].
-        eexists. split; [|eassumption].
-        cbn.
-        cbn in sL; destruct sL as ((?busy, (?done, (?regs, ?d2h))), (?s_tl, ?s_inner));
-            simplify_invariant incr;
-            logical_simplify; tlsimpl; subst.
-        apply No_inflight.
-        simplify_invariant Incr.inner; destruct s_inner; logical_simplify.
-        destruct x as [|[|[|]]]; [exfalso; lia|..| exfalso; lia];
-          destruct_tl_h2d; tlsimpl; subst;
-            match goal with
-            | H: word_to_N v = word_to_N val |- _ =>
-              rewrite <- H
-            end.
-        * constructor; lia.
-        * replace ((word_to_N v + 1) mod 4294967296)%N with
-                        (word_to_N (word.add (word.of_Z 1) v)) by
-              (unfold word_to_N; ZnWords).
-          constructor.
-      + (* [r:=STATUS] *)
-        inversion_rel_spec;
-          try (exfalso; destruct_tl_h2d; tlsimpl; subst; unfold word_to_N in *; cbn in *; ZnWords).
     - (* read_step_unique: *)
       intros. simpl in *. unfold read_step in *. simp.
       destruct v; destruct r; try contradiction; simp; try reflexivity.
